Add support for heterogenous memory injections
I split the injection-related methods from [MemoryOps] and [MemoryStates]
into their own [InjectOps] and [MemoryInjections] classes, which accept
potentially distinct types for the source and target memory states as their
parameters.

The subclass [HeterogenousInjection] handles the special case where they are
identical (otherwise, [inject_neutral] does not make sense).

common/Memtype.v
@@ -185,7 +185,9 @@ drop_perm: forall (m: mem) (b: block) (lo hi: Z) (p: permission), option mem;
 extends: mem -> mem -> Prop;
 
 (** Memory states that inject into themselves. *)
-inject_neutral: forall (thr: block) (m: mem), Prop;
+inject_neutral: forall (thr: block) (m: mem), Prop
+
+}.
 
 (** A memory injection [f] is a function from addresses to either [None]
   or [Some] of an address and an offset.  It defines a correspondence
@@ -200,7 +202,12 @@ inject_neutral: forall (thr: block) (m: mem), Prop;
 
   Likewise, a memory injection [f] defines a relation between memory states 
   that we axiomatize below. *)
-inject: meminj -> mem -> mem -> Prop
+
+Class InjectOps smem tmem
+  `{smem_ops: MemoryOps smem}
+  `{tmem_ops: MemoryOps tmem} := {
+
+inject: meminj -> smem -> tmem -> Prop
 
 }.
 
@@ -243,7 +250,7 @@ Definition inj_offset_aligned (delta: Z) (size: Z) : Prop :=
 Definition flat_inj (thr: block) : meminj :=
   fun (b: block) => if zlt b thr then Some(b, 0) else None.
 
-Class MemoryStates (mem: Type) `{mem_ops: MemoryOps mem} := {
+Class MemorySpec (mem: Type) `{mem_ops: MemoryOps mem} := {
 
 (** * Permissions, block validity, access validity, and bounds *)
 
@@ -926,10 +933,6 @@ perm_free_list:
 
 (** Memory states that inject into themselves. *)
 
-neutral_inject m:
-  inject_neutral (nextblock m) m ->
-  inject (flat_inj (nextblock m)) m m;
-
 empty_inject_neutral thr:
   inject_neutral thr empty;
 
@@ -955,9 +958,14 @@ drop_inject_neutral m b lo hi p m' thr:
 (** This ugly workaround is to prevent the [intuition] tactic from
   destructing instances of MEM which are in the context. *)
 ugly_workaround_dependee: Type;
-ugly_workaround_depender: ugly_workaround_dependee;
+ugly_workaround_depender: ugly_workaround_dependee
+
+}.
 
 (** * Memory injections *)
+
+Class MemoryInjections smem tmem `{inject_ops: InjectOps smem tmem} :=
+{
 
 mi_freeblocks f m1 m2:
   inject f m1 m2 ->
@@ -1231,6 +1239,27 @@ drop_outside_inject f m1 m2 b lo hi p m2':
     perm m1 b' ofs k p -> lo <= ofs + delta < hi -> False) ->
   inject f m1 m2'
 
+}.
+
+Class HomogenousInjections mem
+  `{mem_ops: MemoryOps mem}
+  `{inj_ops: !InjectOps mem mem} :=
+{
+
+homogenous_injecions :> MemoryInjections mem mem;
+
+neutral_inject m:
+  inject_neutral (nextblock m) m ->
+  inject (flat_inj (nextblock m)) m m
+
+}.
+
+Class MemoryStates mem
+  `{mem_ops: MemoryOps mem}
+  `{inj_ops: !InjectOps mem mem} :=
+{
+  memory_states_spec :> MemorySpec mem;
+  memory_states_inject :> HomogenousInjections mem
 }.
 
 End Mem.
